filled some holes

deps/poulet4/lib/P4cub/Transformations/Lifting/Lift.v
@@ -99,6 +99,111 @@ Inductive Lift_e
     (Expr.Lists ls (map fst (shift_pairs shift_e (combine es' ess)))
        :: concat (map snd (shift_pairs shift_e (combine es' ess)))).
 
+Section LifteInduction.
+  Variable P : Expr.e -> Expr.e -> list Expr.e -> Prop.
+
+  Hypothesis HLift_bool : forall (b : bool), P b b [].
+
+  Hypothesis HLift_var : forall t og x,
+      P (Expr.Var t og x) (Expr.Var t og x) [].
+
+  Hypothesis HLift_error : forall err,
+      P (Expr.Error err) (Expr.Error err) [].
+  
+  Hypothesis HLift_bit : forall w n,
+      P (w `W n) (Expr.Var (Expr.TBit w) "" 0) [w `W n].
+
+  Hypothesis HLift_int : forall w z,
+      P (w `S z) (Expr.Var (Expr.TInt w) "" 0) [w `S z].
+  
+  Hypothesis HLift_member : forall t x e e' es,
+      Lift_e e e' es ->
+      P e e' es ->
+      P (Expr.Member t x e) (Expr.Member t x e') es.
+  
+  Hypothesis HLift_uop : forall t o e e' es,
+      Lift_e e e' es ->
+      P e e' es ->
+      P (Expr.Uop t o e) (Expr.Var t "" 0) (Expr.Uop t o e' :: es).
+  
+  Hypothesis HLift_slice : forall hi lo e e' es,
+      Lift_e e e' es ->
+      P e e' es ->
+      P
+        (Expr.Slice hi lo e)
+        (Expr.Var (Expr.TBit (Npos hi - Npos lo + 1)%N) "" 0)
+        (Expr.Slice hi lo e' :: es).
+  
+  Hypothesis HLift_cast : forall t e e' es,
+      Lift_e e e' es ->
+      P e e' es ->
+      P (Expr.Cast t e) (Expr.Var t "" 0) (Expr.Cast t e' :: es).
+  
+  Hypothesis HLift_index : forall t e1 e2 e1' e2' es1 es2,
+      Lift_e e1 e1' es1 ->
+      P e1 e1' es1 ->
+      Lift_e e2 e2' es2 ->
+      P e2 e2' es2 ->
+      P
+        (Expr.Index t e1 e2)
+        (Expr.Index
+           t
+           (shift_e (Shifter 0 (length es2)) e1')
+           (shift_e (Shifter (length es2) (length es1)) e2'))
+        (shift_list shift_e (Shifter 0 (length es1)) es2 ++ es1).
+  
+  Hypothesis HLift_bop : forall t o e1 e2 e1' e2' es1 es2,
+      Lift_e e1 e1' es1 ->
+      P e1 e1' es1 ->
+      Lift_e e2 e2' es2 ->
+      P e2 e2' es2 ->
+      P
+        (Expr.Bop t o e1 e2)
+        (Expr.Var t "" 0)
+        (Expr.Bop
+           t o
+           (shift_e (Shifter 0 (length es2)) e1')
+           (shift_e (Shifter (length es2) (length es1)) e2')
+           :: shift_list shift_e (Shifter 0 (length es1)) es2 ++ es1).
+  
+  Hypothesis HLift_lists : forall ls es es' ess,
+      Forall3 Lift_e es es' ess ->
+      Forall3 P es es' ess ->
+      P
+        (Expr.Lists ls es)
+        (Expr.Var (t_of_lists ls es) "" 0)
+        (Expr.Lists ls (map fst (shift_pairs shift_e (combine es' ess)))
+           :: concat (map snd (shift_pairs shift_e (combine es' ess)))).
+
+  Definition custom_Lift_e_ind : forall e e' es,
+      Lift_e e e' es -> P e e' es :=
+    fix F e e' es hLift :=
+      let fix F3 {es es' : list Expr.e} {ess : list (list Expr.e)}
+            (h : Forall3 Lift_e es es' ess)
+        : Forall3 P es es' ess :=
+        match h with
+        | Forall3_nil _ => Forall3_nil _
+        | Forall3_cons _ _ _ _ _ _ _ h ih
+          => Forall3_cons _ _ _ _ _ _ _ (F _ _ _ h) (F3 ih)
+        end in
+      match hLift with
+      | Lift_bool b => HLift_bool b
+      | Lift_var x y z => HLift_var x y z
+      | Lift_error e => HLift_error e
+      | Lift_bit x y => HLift_bit x y
+      | Lift_int x y => HLift_int x y
+      | Lift_member t x _ _ _ h => HLift_member t x _ _ _ h (F _ _ _ h)
+      | Lift_uop t o _ _ _ h => HLift_uop t o _ _ _ h (F _ _ _ h)
+      | Lift_slice hi lo _ _ _ h => HLift_slice hi lo _ _ _ h (F _ _ _ h)
+      | Lift_cast t _ _ _ h => HLift_cast t _ _ _ h (F _ _ _ h)
+      | Lift_index t _ _ _ _ _ _ h1 h2
+        => HLift_index t _ _ _ _ _ _ h1 (F _ _ _ h1) h2 (F _ _ _ h2)
+      | Lift_bop x y _ _ _ _ _ _ h1 h2
+        => HLift_bop x y _ _ _ _ _ _ h1 (F _ _ _ h1) h2 (F _ _ _ h2)
+      | Lift_lists ls _ _ _ h => HLift_lists ls _ _ _ h (F3 h)
+      end.
+End LifteInduction.
+
 Variant Lift_arg :
   Expr.arg -> Expr.arg -> list Expr.e -> Prop :=
   | Lift_pain e e' es :
@@ -241,36 +346,29 @@ Section Liftlift.
   Lemma Lift_lift_e : forall e e' es,
       Lift_e e e' es -> lift_e e = (e', es).
   Proof.
-    intro e; induction e using custom_e_ind;
-      intros e' le h; inv h; unravel;
+    intros e e' es h;
+      induction h using custom_Lift_e_ind;
+      unravel;
       repeat destr_lift_e;
       repeat match goal with
-        | ih: (forall e' es, Lift_e ?e e' es -> (_, _) = (e', es)), h: Lift_e ?e _ _
-          |- _ => apply ih in h; inv h; clear ih
+        | h: (_, _) = (_, _) |- _ => inv h
         end; auto.
-    destruct (split (shift_pairs shift_e (map lift_e exps)))
+    destruct (split (shift_pairs shift_e (map lift_e es)))
       as [es'' les] eqn:hsplit.
     rewrite split_map in hsplit. inv hsplit.
-    enough (map lift_e exps = combine es' ess) as h.
+    enough (map lift_e es = combine es' ess) as h.
     { do 5 f_equal; assumption. }
-    assert (h12 : length exps = length es') by eauto using Forall3_length12.
-    pose proof Forall_specialize_Forall2
-      _ _ _ _ H _ h12 as h; clear H.
-    assert (h23 : length es' = length ess) by eauto using Forall3_length23.
-    pose proof Forall2_specialize_Forall3
-      _ _ _ _ _ _ h _ h23 as ih; clear h.
-    pose proof Forall3_impl_Forall3
-      _ _ _ _ _ _ _ _ ih H4 as h; clear ih.
+    assert (h12 : length es = length es') by eauto using Forall3_length12.
     rewrite Forall3_map_1 with
       (R:=fun e e' es => e = (e', es))
-      (f:=lift_e) in h.
-    rewrite Forall3_Forall2_combine_r in h.
-    destruct h as [_ h].
+      (f:=lift_e) in H0.
+    rewrite Forall3_Forall2_combine_r in H0.
+    destruct H0 as [_ h].
     rewrite <- Forall2_eq.
     rewrite Forall2_forall_nth_error in h |- *.
     destruct h as [hlen h].
     split; try assumption.
-    intros n [e es] [e' es''] H H'.
+    intros n [e Es] [e' es''] Hyp H'.
     firstorder.
   Qed.
 
